\begin{eqnarray}
\Lagr & = & \frac{1}{4}G_{\mu\nu}^{A}G^{\mu\nu A} + \frac{1}{4}W_{\mu\nu}^{a}W^{\mu\nu a} + \frac{1}{4}B_{\mu\nu}B^{\mu\nu} \\
      & + & i\overline{l}_{L}^{i}Dl_{L}^{i} + i\overline{q}_{L}^{i}Dq_{L}^{i} + i\overline{e}_{R}^{i}De_{R}^{i} + i\overline{u}_{R}^{i}Du_{R}^{i}  + i\overline{d}_{R}^{i}Dd_{R}^{i} \\
      & + & (D_{\mu}\phi)^{\dagger}D_{\mu}\phi - V(\phi) - \left(y_{ii}^{e}\overline{l}_{L}^{i}\phi e_{R}^{i} + y_{ii}^{d}\overline{q}_{L}^{i}\phi d_{R}^{i} + V_{ij}y_{jj}^{u}\overline{q}_{L}^{i}\phi u_{R}^{j} + h.c.\right)
\end{eqnarray}

\begin{equation}
D_{\mu} = \partial_{\mu} + ig_{s}G_{\mu}^{A}T_{A} + igW_{\mu}^{a}T_{a} + ig^{\prime}B_{\mu}Y
\end{equation}

\begin{eqnarray}
G_{\mu\nu}^{A} & = & \partial_{\mu}G_{\nu}^{A} - \partial_{\nu}G_{\mu}^{A} - g_{s}f_{BC}^{A}G_{\mu}^{B}G_{\nu}^{C} \\
W_{\mu\nu}^{a} & = & \partial_{\mu}W_{\nu}^{a} - \partial_{\nu}W_{\mu}^{A} - g\epsilon^{abc}W_{\mu}^{b}W_{\nu}^{c} \\
B_{\mu\nu}     & = & \partial_{\mu}B_{\nu} - \partial_{\nu}B_{\mu}
\end{eqnarray}

\begin{equation}
q_{L}^{i} = \begin{pmatrix}u_{L}^{i} \\ d_{L}^{i}\end{pmatrix} \sim (3,2)_{\frac{1}{6}}, u_{R}^{i} \sim (3,1)_{\frac{2}{3}}, u_{R}^{i} \sim (3,1)_{\frac{1}{3}}
\end{equation}

\begin{equation}
l_{L}^{i} = \begin{pmatrix}\nu_{L}^{i} \\ e_{L}^{i}\end{pmatrix} \sim (1,2)_{-\frac{1}{2}}, e_{R}^{i} \sim (1,1)_{-1}
\end{equation}

\begin{equation}
\phi = \begin{pmatrix}\phi^{+} \\ \phi^{0}\end{pmatrix} \sim (1,2)_{\frac{1}{2}}
\end{equation}

\begin{equation}
V(\phi) = \mu^{2}|\phi|^{2} + \lambda|\phi|^{4}
\end{equation}

\begin{equation}
W_{\mu}^{\pm}=\frac{1}{\sqrt{2}}(W_{\mu}^{1} \mp iW_{\mu}^{2}),                       m_{W}=g\frac{v}{2}
\end{equation}

\begin{equation}
Z_{\mu}^{0}  =\frac{1}{\sqrt{g^{2} + g^{\prime 2}}}(gW_{\mu}^{3} - g^{\prime}B_{\mu}),m_{Z}=\sqrt{g^{2} + g^{\prime 2}}\frac{v}{2}
\end{equation}

\begin{equation}
A_{\mu} = \frac{1}{\sqrt{g^{2} + g^{\prime 2}}}(g^{\prime} A_{\mu}^{3} + gB_{\mu}).
\end{equation}
